fiat2/src/fiat2/PipelineEx.v
@@ -63,13 +63,6 @@ Section ConcreteExample.
     fun tbl => fold_command_with_globals [tbl]
                  (filter_to_bitmap_lookup_head bitmap_attr bitmap_str "id_tag" "aux_tag" "pk_idx_tag" "bm_tag" "x" "b" "acc" tbl).
 
-  Hint Extern 5 (type_of _ _ IndexInterface2.to_idx _) => apply SumAgg.to_idx_ty : transf_hints.
-  Hint Extern 5 (type_of _ _ IndexInterface2.to_idx _) => apply DictIndexImpl2.to_idx_ty : transf_hints.
-  Hint Extern 5 (type_of _ _ IndexInterface2.to_idx _) => apply BitmapIndex.to_pk_idx_ty : transf_hints.
-  Hint Extern 5 (type_of _ _ IndexInterface2.to_idx _) => apply BitmapIndex.to_bitmap_ty : transf_hints.
-  Hint Extern 5 (type_wf (IndexInterface2.idx_ty _)) => apply DictIndexImpl2.idx_ty_wf : transf_hints.
-  Hint Extern 5 (type_wf (IndexInterface2.idx_ty _)) => apply BitmapIndex.pk_idx_ty_wf : transf_hints.
-
   Notation idxs := [("sum_agg_tag", csum_agg, sum_agg_wf);
                     ("dict_idx_tag", cdict_idx, dict_idx_wf);
                     ("pk_idx_tag", cpk_idx, pk_idx_wf);
@@ -79,91 +72,6 @@ Section ConcreteExample.
   apply compo_idx_ok; repeat constructor; intros; auto with transf_hints.
   all: cbn; rewrite <- eqb_eq; intuition idtac; discriminate.
   Qed.
-
-  (* ??? move to TransfUtils *)
-  Fixpoint repeat_transf (f : command -> command) (n : nat) :=
-    match n with
-    | O => id
-    | S n => Basics.compose f (repeat_transf f n)
-    end.
-
-  Section repeat_transf_sound.
-    Context {tenv : map.map string type} {tenv_ok : map.ok tenv}.
-    Context {locals : map.map string value} {locals_ok : map.ok locals}.
-
-    Lemma repeat_transf_preserve_aug_transf_sound : forall is_tbl_ty aux_ty aux_wf f n,
-        aug_transf_sound is_tbl_ty aux_ty aux_wf f ->
-        aug_transf_sound (locals:=locals) is_tbl_ty aux_ty aux_wf (fun tbl => repeat_transf (f tbl) n).
-    Proof.
-      induction n; cbn.
-      1:{ intros _. unfold aug_transf_sound; auto. }
-      1:{ intros; cbn. apply aug_transf_sound_compose; auto. }
-    Qed.
-  End repeat_transf_sound.
-
-  Ltac apply_transf_sound_lemmas :=
-    lazymatch goal with
-    | |- transf_sound (apply_idx_related_transfs _ _ _) => apply apply_idx_related_transfs_sound
-    | |- aug_transf_sound _ _ _ (fun _ => Basics.compose _ _) => apply aug_transf_sound_compose
-    | |- transf_sound (fun _ _ => Basics.compose _ _) => apply transf_sound_compose
-    | |- aug_transf_sound _ _ _ (fun _ => repeat_transf _ _) => apply repeat_transf_preserve_aug_transf_sound
-    | |- aug_transf_sound _ _ _ _ => apply fold_command_with_globals_sound
-    | |- transf_sound ?x => unfold x
-    end.
-
-  Hint Extern 5 ((_ : string) <> _) => apply eqb_neq; auto : transf_hints.
-  Hint Resolve push_down_collection_sound : transf_hints.
-  Hint Resolve annotate_collection_sound : transf_hints.
-  Hint Extern 5 (forall v, aux_wf _ _ v -> SumAgg.aux_wf_for_idx _ _ _ _ _ _ v) =>
-              intros; unfold aux_wf, aux_wf_for_idx, compo_idx_wf in *;
-              repeat destruct_match_hyp; intuition idtac;
-              repeat invert_Forall; unfold SumAgg.idx_wf, record_proj in *;
-                             destruct_match_hyp; intuition eauto : transf_hints.
-  Hint Extern 5 (SumAgg.aux_ty_for_idx _ _ _ _) => unfold SumAgg.aux_ty_for_idx, aux_ty; cbn; auto : transf_hints.
-  Hint Extern 5 (forall t, IndexInterface2.is_tbl_ty t = true -> _ = true) =>
-         unfold IndexInterface2.is_tbl_ty; cbn; intros;
-  rewrite !Bool.andb_true_iff in *; intuition auto : transf_hints.
-  Hint Resolve cons_to_add_head_sound : transf_hints.
-  Hint Resolve sum_to_agg_lookup_head_sound : transf_hints.
-  Hint Resolve cons_to_insert_head_sound : transf_hints.
-  Hint Resolve cons_to_pk_idx_update_head_sound : transf_hints.
-  Hint Resolve cons_to_bitmap_update_head_sound : transf_hints.
-  Hint Resolve use_bitmap_head_sound : transf_hints.
-  Hint Resolve use_idx_head_sound2 : transf_hints.
-  Hint Resolve eq_filter_to_lookup_head_sound2 : transf_hints.
-  Hint Resolve filter_to_bitmap_lookup_head_sound2 : transf_hints.
-  Hint Resolve use_pk_idx_head_sound2 : transf_hints.
-  (*
-  Hint Extern 5 (expr_aug_transf_sound _ _ _ (DictIndexImpl2.use_idx_head _ _ _ _)) =>
-         eapply use_idx_head_sound; [ | | | | | | eauto with transf_hints ]; auto with transf_hints : transf_hints.
-  Hint Extern 5 (expr_aug_transf_sound _ _ _ (DictIndexImpl2.eq_filter_to_lookup_head _ _ _ _ _)) =>
-         eapply eq_filter_to_lookup_head_sound; [ | | | | | | eauto with transf_hints ]; auto with transf_hints : transf_hints.
-  Hint Extern 5 (expr_aug_transf_sound IndexInterface2.is_tbl_ty _ _
-                   (filter_to_bitmap_lookup_head _ _ _ _ _ _ _ _ _)) =>
-         eapply filter_to_bitmap_lookup_head_sound; eauto with transf_hints; auto with transf_hints : transf_hints.
-  Hint Extern 5 (expr_aug_transf_sound IndexInterface2.is_tbl_ty _ _
-                         (use_pk_idx_head _ _ _)) =>
-          eapply use_pk_idx_head_sound; eauto with transf_hints; auto with transf_hints : transf_hints. *)
-  Hint Extern 5 (forall v, aux_wf _ _ v -> DictIndexImpl2.aux_wf_for_idx _ _ _ _ _ _ _ _ v) =>
-         intros; unfold aux_wf, DictIndexImpl2.aux_wf_for_idx, compo_idx_wf in *;
-                 repeat destruct_match_hyp; intuition idtac;
-  repeat invert_Forall; unfold DictIndexImpl2.idx_wf, record_proj in *;
-                        destruct_match_hyp; intuition eauto : transf_hints.
-  Hint Extern 5 (forall v, aux_wf _ _ v -> SumAgg.aux_wf_for_idx _ _ _ _ _ _ v) =>
-         intros; unfold aux_wf, SumAgg.aux_wf_for_idx, compo_idx_wf in *;
-                 repeat destruct_match_hyp; intuition idtac;
-  repeat invert_Forall; unfold SumAgg.idx_wf, record_proj in *;
-                        destruct_match_hyp; intuition eauto : transf_hints.
-  Hint Extern 5 (forall v, aux_wf _ _ v -> BitmapIndex.aux_wf_for_idx _ _ _ _ v) =>
-         intros; unfold aux_wf, BitmapIndex.aux_wf_for_idx, compo_idx_wf in *;
-                 repeat destruct_match_hyp; intuition idtac;
-  repeat invert_Forall; unfold BitmapIndex.bitmap_wf, record_proj in *;
-            destruct_match_hyp; intuition eauto : transf_hints.
-  (* ??? Simplify this? ^^^ *)
-  Hint Extern 5 (DictIndexImpl2.aux_ty_for_idx _ _ _ _ _) => unfold DictIndexImpl2.aux_ty_for_idx, aux_ty; cbn; auto : transf_hints.
-  Hint Extern 5 (BitmapIndex.aux_ty_for_idx _ _ _ _ _) => unfold BitmapIndex.aux_ty_for_idx, aux_ty; cbn; auto : transf_hints.
- (* Hint Unfold ??? *)
-  Hint Extern 5 string => exact ("":string).
 
   Definition ex_transf (Gstore Genv : ctenv) :=
     Basics.compose
@@ -187,21 +95,23 @@ Section ConcreteExample.
 
   Lemma ex_transf_sound : transf_sound (locals:=clocals) ex_transf.
   Proof.
-    repeat (repeat apply_transf_sound_lemmas; eauto with transf_hints).
+    repeat (repeat apply_transf_sound_lemmas; eauto 10 with transf_hints).
   Qed.
 
   Require Import fiat2.Notations.
   Open Scope fiat2_scope.
 
   Definition row_ty := TRecord (record_sort [("name", TString); ("department", TString); ("feedback", TString); ("salary", TInt); ("state", TString)]).
-  (* Two Arbitrary Well_typed rows *)
+  (* Two Arbitrary well_typed rows *)
   Definition row1 := EVar "row1".
   Definition row2 := EVar "row2".
+  (* ??? change the names *)
 
   Definition build_responses1 := <{ set "responses" := row1 :: row2 :: mut "responses" }>.
   Definition filter_responses dpt : expr := ESort LikeList <[ "row" <- mut "responses" ;
                                                        check("row"["department"] == << EAtom (AString dpt) >>);
                                                               ret "row" ]>.
+  (* ??? foreach from another table to update this table e.g. purchase of items*)
   Definition filter_responses2 : expr := <[ "row" <- mut "responses" ;
                                             check("row"["state"] == << EAtom (AString "MA") >>);
                                             ret "row" ]>.
@@ -228,21 +138,12 @@ Section ConcreteExample.
   Definition ex1_transformed := ex_transf init_Gstore init_Genv ex1.
   Compute ex1_transformed.
 
-  Ltac resolve_NoDup := repeat constructor; simpl; intuition idtac; congruence.
-
-  Ltac resolve_tenv_wf := repeat apply tenv_wf_step; try apply tenv_wf_empty; repeat constructor; resolve_NoDup.
-
-  Hint Extern 5 (well_typed _ _ _) => simple eapply command_typechecker_sound.
-  Hint Extern 5 (tenv_wf _) => resolve_tenv_wf.
-  Hint Extern 5 (typecheck _ _ _ = Success _) => reflexivity.
-
   Theorem ex1_transformed_sem : forall (store env : clocals),
       locals_wf init_Gstore store ->
       locals_wf init_Genv env ->
       interp_command store env ex1_transformed = interp_command store env ex1.
   Proof.
-    intros. apply transf_sound__preserve_sem; auto using ex_transf_sound.
-    (* ??? debug eauto 2 using transf_sound__preserve_sem, ex_transf_sound. *)
+    intros. apply transf_sound__preserve_sem; auto using ex_transf_sound with transf_hints.
   Qed.
 End ConcreteExample.
 
